thys/EdmondsKarp_Maxflow/Augmenting_Path_BFS.thy
@@ -1,7 +1,6 @@
 section \<open>Breadth First Search\<close>
 theory Augmenting_Path_BFS
 imports Refine_Add_Fofu Graph_Impl 
-  Refine_Monadic_Syntax_Sugar
 begin
   text \<open>
     In this theory, we present a verified breadth-first search
