thys/EdmondsKarp_Maxflow/Fofu_Impl_Base.thy
@@ -3,7 +3,6 @@ imports
   "../Refine_Imperative_HOL/IICF/IICF"
   "../Refine_Imperative_HOL/Sepref_ICF_Bindings"
   "~~/src/HOL/Library/Rewrite"
-  Refine_Monadic_Syntax_Sugar
 begin
   hide_type (open) List_Seg.node
 
